Tactics.v
@@ -1,122 +1,5 @@
 Require Import Lib.EclecticLib Syntax Properties.
 
-Ltac discharge_string_dec :=
-  repeat match goal with
-         | |- context[string_dec ?P ?Q] => destruct (string_dec P Q);
-                                           discharge_appendage;
-                                           try (tauto || congruence)
-         end.
-
-Ltac discharge_SemAction :=
-  repeat match goal with
-         | |- SemAction _ (If ?p then _ else _ as _; _)%kami_action _ _ _ _ => eapply SemAction_if
-         | |- if ?P then SemAction _ _ _ _ _ _ else SemAction _ _ _ _ _ _ => case_eq P; let H := fresh in intros H; rewrite ?H in *; try discriminate
-         | |- SemAction _ (convertLetExprSyntax_ActionT _) _ _ _ _ => eapply convertLetExprSyntax_ActionT_same
-         | |- SemAction _ _ _ _ _ _ => econstructor
-         end; rewrite ?key_not_In_fst in *; simpl in *; try tauto; simpl in *; unfold not; intros; rewrite ?DisjKeyWeak_same by apply string_dec;
-  unfold DisjKeyWeak; intros; simpl in *;
-  repeat match goal with
-         | H: _ \/ _ |- _ => destruct H; discharge_appendage
-         | H: False |- _ => exfalso; apply H
-         | H: ?a = ?b |- _ => match type of a with
-                              | string => try discriminate
-                              end
-         end.
-
-Local Example test_normaldisj:
-  DisjKey (map (fun x => (x, 1)) ("a" :: "b" :: "c" :: nil))%string
-          (map (fun x => (x, 2)) ("d" :: "e" :: nil))%string.
-Proof.
-  simpl.
-  discharge_DisjKey.
-Qed.
-
-Local Example test_prefix_disj a:
-  DisjKey (map (fun x => ((a ++ x)%string, 1)) ("ab" :: "be" :: "cs" :: nil))%string
-          (map (fun x => ((a ++ x)%string, 2)) ("de" :: "et" :: nil))%string.
-Proof.
-  simpl.
-  discharge_DisjKey.
-Qed.
-
-Local Example test_suffix_disj a:
-  DisjKey (map (fun x => ((x ++ a)%string, 1)) ("ab" :: "be" :: "cs" :: nil))%string
-          (map (fun x => ((x ++ a)%string, 2)) ("de" :: "et" :: nil))%string.
-Proof.
-  simpl.
-  discharge_DisjKey.
-Qed.
-
-Local Ltac clean_hyp :=
-  repeat match goal with
-         | H: @key_not_In _ _ _ _ |- _ => clear H
-         end;
-  repeat match goal with
-         | H: DisjKey _ _ |- _ => apply DisjKeyWeak_same in H; [unfold DisjKeyWeak in H; simpl in H| apply string_dec]
-         | H: In ?x ?ls |- _ =>
-           apply (InFilter string_dec) in H; simpl in H; destruct H; [|exfalso; auto]
-         | H: False |- _ => exfalso; apply H
-         | H: (?A, ?B) = (?P, ?Q) |- _ =>
-           let H1 := fresh in
-           let H2 := fresh in
-           pose proof (f_equal fst H) as H1;
-           pose proof (f_equal snd H) as H2;
-           simpl in H1, H2;
-           clear H
-         | H: ?A = ?A |- _ => clear H
-         | H: (?a ++ ?b)%string = (?a ++ ?c)%string |- _ => rewrite append_remove_prefix in H; subst
-         | H: (?a ++ ?b)%string = (?c ++ ?b)%string |- _ => rewrite append_remove_suffix in H; subst
-         | H: existT ?a ?b ?c1 = existT ?a ?b ?c2 |- _ => apply Eqdep.EqdepTheory.inj_pair2 in H; subst
-         | H: ?A = ?B |- _ => discriminate
-         | H: SemAction _ (convertLetExprSyntax_ActionT ?e) _ _ _ _ |- _ =>
-           apply convertLetExprSyntax_ActionT_full in H; dest; subst
-         end.
-
-Local Ltac destruct_RegT :=
-  repeat match goal with
-         | H: RegT |- _ =>
-           destruct H as [? [? ?]]; simpl in *; repeat subst; simpl in *
-         end.
-
-Local Ltac destruct_Invariant mySimRel :=
-  try match goal with
-      | H: mySimRel _ _ |- _ => inv H
-      end; clean_hyp.
-
-Local Ltac discharge_init :=
-  repeat econstructor; eauto; simpl;
-  instantiate (1 := eq_refl); simpl; auto.
-
-Ltac discharge_simulationZero mySimRel :=
-  apply simulationZeroAction with (simRel := mySimRel); auto; simpl; intros; destruct_Invariant mySimRel; auto;
-  (repeat match goal with
-          | H: _ \/ _ |- _ => destruct H
-          | H: False |- _ => exfalso; apply H
-          | H: (?a, ?b) = (?c, ?d) |- _ =>
-            let H2 := fresh in
-            inversion H;
-            pose proof (f_equal snd H) as H2;
-            simpl in H2; subst; clear H; EqDep_subst
-         | H: SemAction _ (convertLetExprSyntax_ActionT ?e) _ _ _ _ |- _ =>
-           apply convertLetExprSyntax_ActionT_full in H; dest; subst
-          | H: SemAction _ _ _ _ _ _ |- _ =>
-            apply inversionSemAction in H; dest; subst
-          | H: if ?P then _ else _ |- _ => case_eq P; let i := fresh in intros i; rewrite ?i in *; dest
-          | H: Forall2 _ _ _ |- _ => inv H
-          | H: ?a = ?a |- _ => clear H
-          | H: match convertLetExprSyntax_ActionT ?P with
-               | _ => _
-               end |- _ =>
-            case_eq P; intros;
-            match goal with
-            | H': P = _ |- _ => rewrite ?H' in *; simpl in *; try discriminate
-            end
-          end); dest; simpl in *; repeat subst; simpl in *; destruct_RegT;
-  match goal with
-  | |- exists rspec, _ => discharge_init
-  | _ => idtac
-  end.
-
 Ltac discharge_NoSelfCall :=
   unfold NoSelfCallBaseModule, NoSelfCallRulesBaseModule, NoSelfCallMethsBaseModule; split; auto; simpl; intros;
   repeat match goal with
@@ -127,7 +10,7 @@ Ltac discharge_NoSelfCall :=
          end.
 
 Ltac discharge_simulationGeneral mySimRel disjReg :=
-  apply simulationGeneral with (simRel := mySimRel); auto; simpl; intros; destruct_Invariant mySimRel; auto;
+  apply simulationGeneral with (simRel := mySimRel); auto; simpl; intros;
   (repeat match goal with
           | H: _ \/ _ |- _ => destruct H
           | H: False |- _ => exfalso; apply H
@@ -152,185 +35,217 @@ Ltac discharge_simulationGeneral mySimRel disjReg :=
             match goal with
             | H': P = _ |- _ => rewrite ?H' in *; simpl in *; try discriminate
             end
-          end); dest; simpl in *; repeat subst; simpl in *; destruct_RegT;
-  match goal with
-  | |- exists rspec, _ => discharge_init
-  | _ => idtac
-  end.
+          end); dest; simpl in *; repeat subst; simpl in *.
 
-
-
-
-
-Notation sz := 5.
-
-Section Named.
-  Variable name: string.
-  Local Notation "^ x" := (name ++ "." ++ x)%string (at level 0).
-
-    Definition IncrementerImpl :=
-      MODULE_WF {
-          Register ^"counter" : Bit sz <- Default
-            with Register ^"counter1" : Bit sz <- Default
-            with Register ^"isSending" : Bool <- true
-                                             
-            with Rule ^"send" :=
-            ( Read isSending: Bool <- ^"isSending" ;
-                Assert #isSending ;
-                Read counter: Bit sz <- ^"counter" ;
-                Call "counterVal"(#counter: _);
-                Write ^"isSending" <- !#isSending ;
-                Retv )
-
-            with Rule ^"inc" :=
-              ( Read isSending: Bool <- ^"isSending" ;
-                  Assert !#isSending ;
-                  Read counter: Bit sz <- ^"counter" ;
-                  Write ^"counter" <- #counter + $1;
-                  Write ^"isSending" <- !#isSending ;
-                  Retv )
-        }.
-
-  Definition IncrementerSpec :=
-    MODULE_WF {
-        Register ^"counter" : Bit sz <- Default
-          with Register ^"counter1" : Bit sz <- Default
-                                         
-          with Rule ^"send_and_inc" :=
-          ( Read counter: Bit sz <- ^"counter" ;
-              Call "counterVal"(#counter: _);
-              Write ^"counter" <- #counter + $1;
-              Retv)
-      }.
-
-  Record Incrementer_invariant (impl spec: RegsT) : Prop :=
-    { counterImpl: word sz ;
-      isSending: bool ;
-      implEq : impl = (^"counter", existT _ (SyntaxKind (Bit sz)) counterImpl)
-                        :: (^"counter1", existT _ (SyntaxKind (Bit sz)) $0)
-                        :: (^"isSending", existT _ (SyntaxKind Bool) isSending) :: nil ;
-      specEq : spec = (^"counter", existT _ (SyntaxKind (Bit sz))
-                                         (if isSending then counterImpl else counterImpl ^+ $1))
-                        :: (^"counter1", existT  _ (SyntaxKind (Bit sz)) $0)
-                        :: nil
-    }.
-End Named.
-
-(*
-Theorem Incrementer_TraceInclusion (name: string) :
-  TraceInclusion (Base (IncrementerImpl name)) (Base (IncrementerSpec name)).
-Proof.
-  apply simulationZeroAction with (simRel := (Incrementer_invariant name)); auto; simpl; intros; destruct_Invariant (Incrementer_invariant name); auto.
-  (repeat match goal with
-          | H: _ \/ _ |- _ => destruct H
-          | H: False |- _ => exfalso; apply H
-          | H: (?a, ?b) = (?c, ?d) |- _ =>
-            let H2 := fresh in
-            inversion H;
-            pose proof (f_equal snd H) as H2;
-            simpl in H2; subst; clear H; EqDep_subst
+Ltac clean_hyp :=
+  simpl in *;
+  repeat match goal with
+         | H: DisjKey _ _ |- _ => apply DisjKeyWeak_same in H; [unfold DisjKeyWeak in H; simpl in H| apply string_dec]
+         (* | H: In ?x ?ls |- _ => *)
+         (*   apply (InFilterPair string_dec) in H; simpl in H; destruct H; [|exfalso; auto] *)
+         | H: _ \/ _ |- _ => destruct H; subst
+         | H: False |- _ => exfalso; apply H
+         | H: (?A, ?B) = (?P, ?Q) |- _ =>
+           let H1 := fresh in
+           let H2 := fresh in
+           pose proof (f_equal fst H) as H1;
+           pose proof (f_equal snd H) as H2;
+           simpl in H1, H2;
+           clear H
+         | H: ?A = ?A |- _ => clear H
+         | H: (?a ++ ?b)%string = (?a ++ ?c)%string |- _ => rewrite append_remove_prefix in H; subst
+         | H: (?a ++ ?b)%string = (?c ++ ?b)%string |- _ => rewrite append_remove_suffix in H; subst
+         | H: existT ?a ?b ?c1 = existT ?a ?b ?c2 |- _ => apply Eqdep.EqdepTheory.inj_pair2 in H; subst
+         | H: ?A = ?B |- _ => discriminate
          | H: SemAction _ (convertLetExprSyntax_ActionT ?e) _ _ _ _ |- _ =>
            apply convertLetExprSyntax_ActionT_full in H; dest; subst
-          | H: SemAction _ _ _ _ _ _ |- _ =>
-            apply inversionSemAction in H; dest; subst
-          | H: if ?P then _ else _ |- _ => case_eq P; let i := fresh in intros i; rewrite ?i in *; dest
-          | H: Forall2 _ _ _ |- _ => inv H
-          | H: ?a = ?a |- _ => clear H
-          | H: match convertLetExprSyntax_ActionT ?P with
-               | _ => _
-               end |- _ =>
-            case_eq P; intros;
-            match goal with
-            | H': P = _ |- _ => rewrite ?H' in *; simpl in *; try discriminate
-            end
-          end); dest; simpl in *; repeat subst; simpl in *; destruct_RegT.
-  match goal with
-  | |- exists rspec: list RegT, _ => discharge_init
-  | _ => idtac
-  end.
-  (repeat match goal with
-          | H: In ?x ?ls |- _ =>
-            apply (InFilter string_dec) in H; simpl in H; destruct H; [|exfalso; auto]
-          | H: _ \/ _ |- _ => destruct H
-          | H: False |- _ => exfalso; apply H
-          | H: (?a, ?b) = (?c, ?d) |- _ =>
-            let H2 := fresh in
-            inversion H;
-            pose proof (f_equal snd H) as H2;
-            simpl in H2; subst; clear H; EqDep_subst
-          | H: SemAction _ (convertLetExprSyntax_ActionT ?e) _ _ _ _ |- _ =>
-           apply convertLetExprSyntax_ActionT_full in H; dest; subst
-          | H: SemAction _ _ _ _ _ _ |- _ =>
-            apply inversionSemAction in H; dest; subst
-          | H: if ?P then _ else _ |- _ => case_eq P; let i := fresh in intros i; rewrite ?i in *; dest
-          | H: Forall2 _ _ _ |- _ => inv H
-          | H: ?a = ?a |- _ => clear H
-          | H: match convertLetExprSyntax_ActionT ?P with
-               | _ => _
-               end |- _ =>
-            case_eq P; intros;
-            match goal with
-            | H': P = _ |- _ => rewrite ?H' in *; simpl in *; try discriminate
-            end
-          end).
-  match goal with
-  | H: In ?x ?ls |- _ =>
-    apply (InFilter string_dec) in H; simpl in H; try (destruct H; [|exfalso; auto])
-  end.
-  dest; simpl in *; repeat subst; simpl in *; destruct_RegT.
-  
-  - repeat econstructor; eauto; simpl;
-    instantiate (1 := eq_refl); simpl; auto.
-    repeat match goal with
-           | |- match ?pf in _ = Y return (fullType type Y) with
-                | eq_refl => ?P
-                end = ?P => instantiate (1 := eq_refl)
-           end.
-    instantiate (1 := eq_refl); simpl; auto.
-    econstructor; eauto; simpl; auto.
-    econstructor; eauto; simpl; auto.
-    econstructor; eauto; simpl; auto.
-    econstructor; eauto; simpl; auto.
-    Focus 2.
-    match goal with
-    | |- exists pf: _ = _, _ => exists eq_refl
-    end.
-            
-    simpl.
-    constructor.
-    destruct x; simpl in *; subst.
-    destruct x0; simpl in *; subst.
-    destruct s0; simpl in *; repeat subst. subst.
-    destruct x2.
-    match goal with
-    | H: match ?x in (_ = Y) return fullType type Y with
-         | eq_refl => projT2 _
-         end = _ |- _ => destruct x
-    end.
+         end.
 
-    (* Initial values *)
-    destruct x, x0, s0, s2; simpl in *; subst; subst.
-    exists (("counter", existT _ (SyntaxKind (Bit sz)) (wzero 5)) :: nil); simpl in *.
-    split.
-    + repeat constructor; simpl.
-      exists eq_refl; auto.
-    + apply Build_Incrementer_invariant with (counterImpl := (wzero 5)) (isSending := true); auto.
-  - (* Rule send - corresponds to rule send_and_inc in Spec, so "right" *)
-    right; do 2 eexists; repeat split; eauto; simpl in *.
-    inv H1.
-    clean_hyp.
-    do 2 eexists; repeat split; eauto; simpl in *.
-    + discharge_SemAction.
-    + econstructor; eauto; simpl.
-      repeat f_equal.
-      apply wzero_wplus.
-  - (* Rule inc - corresponds to nothing in Spec, so "left" *)
-    left; split; auto; simpl in *.
-    inv H1.
-    clean_hyp.
-    discharge_string_dec.
-    rewrite negb_true_iff in *; subst.
-    econstructor; repeat (simpl; eauto).
-    rewrite wzero_wplus; auto.
-Qed.
-*)
+Ltac discharge_string_dec :=
+  repeat match goal with
+         | |- context[string_dec ?P ?Q] => destruct (string_dec P Q);
+                                           discharge_appendage;
+                                           try (tauto || congruence)
+         end.
+
+Ltac discharge_SemAction :=
+  repeat match goal with
+         | |- SemAction _ (If ?p then _ else _ as _; _)%kami_action _ _ _ _ => eapply SemAction_if
+         | |- if ?P then SemAction _ _ _ _ _ _ else SemAction _ _ _ _ _ _ => case_eq P; let H := fresh in intros H; rewrite ?H in *; try discriminate
+         | |- SemAction _ (convertLetExprSyntax_ActionT _) _ _ _ _ => eapply convertLetExprSyntax_ActionT_same
+         | |- SemAction _ _ _ _ _ _ => econstructor
+         end; rewrite ?key_not_In_fst in *; simpl in *; try tauto; simpl in *; unfold not; intros; rewrite ?DisjKeyWeak_same by apply string_dec;
+  unfold DisjKeyWeak; intros; simpl in *;
+  repeat match goal with
+         | H: _ \/ _ |- _ => destruct H; discharge_appendage
+         | H: False |- _ => exfalso; apply H
+         | H: ?a = ?b |- _ => match type of a with
+                              | string => try discriminate
+                              end
+         end.
+
+(* Ltac discharge_SemAction := *)
+(*   (repeat match goal with                              *)
+(*           | H: SemAction _ (convertLetExprSyntax_ActionT ?e) _ _ _ _ |- _ => *)
+(*             apply convertLetExprSyntax_ActionT_full in H; dest; subst *)
+(*           | H: SemAction _ _ _ _ _ _ |- _ => *)
+(*             apply inversionSemAction in H; dest; subst *)
+(*           | H: if ?P then _ else _ |- _ => case_eq P; let i := fresh in intros i; rewrite ?i in *; dest *)
+(*           | H: key_not_In _ _ |- _ => clear H *)
+(*           | H: DisjKey _ _ |- _ => clear H *)
+(*           end); *)
+(*   repeat match goal with *)
+(*          | H: In (?a, _) ?ls |- _ => *)
+(*            let HF := fresh in *)
+(*            rewrite (InFilterPair string_dec) in H; simpl in H; discharge_append; *)
+(*            apply InSingleton_impl in H; subst *)
+(*          | H: ?a = ?a |- _ => clear H *)
+(*          | H: ?a <> ?a |- _ => exfalso; apply (H eq_refl) *)
+(*          | H: (_, existT _ _ _) = (_, existT _ _ _) |- _ => *)
+(*            apply inversionExistT in H; destruct H as [? ?] *)
+(*          | H: existT ?a ?b ?c1 = existT ?a ?b ?c2 |- _ => apply Eqdep.EqdepTheory.inj_pair2 in H; subst *)
+(*          | H: ?a <> ?b |- _ => clear H *)
+(*          end. *)
+
+(* Local Ltac clean_hyp := *)
+(*   repeat match goal with *)
+(*          | H: @key_not_In _ _ _ _ |- _ => clear H *)
+(*          end; *)
+(*   repeat match goal with *)
+(*          | H: DisjKey _ _ |- _ => apply DisjKeyWeak_same in H; [unfold DisjKeyWeak in H; simpl in H| apply string_dec] *)
+(*          | H: In ?x ?ls |- _ => *)
+(*            apply (InFilterPair string_dec) in H; simpl in H; destruct H; [|exfalso; auto] *)
+(*          | H: False |- _ => exfalso; apply H *)
+(*          | H: (?A, ?B) = (?P, ?Q) |- _ => *)
+(*            let H1 := fresh in *)
+(*            let H2 := fresh in *)
+(*            pose proof (f_equal fst H) as H1; *)
+(*            pose proof (f_equal snd H) as H2; *)
+(*            simpl in H1, H2; *)
+(*            clear H *)
+(*          | H: ?A = ?A |- _ => clear H *)
+(*          | H: (?a ++ ?b)%string = (?a ++ ?c)%string |- _ => rewrite append_remove_prefix in H; subst *)
+(*          | H: (?a ++ ?b)%string = (?c ++ ?b)%string |- _ => rewrite append_remove_suffix in H; subst *)
+(*          | H: existT ?a ?b ?c1 = existT ?a ?b ?c2 |- _ => apply Eqdep.EqdepTheory.inj_pair2 in H; subst *)
+(*          | H: ?A = ?B |- _ => discriminate *)
+(*          | H: SemAction _ (convertLetExprSyntax_ActionT ?e) _ _ _ _ |- _ => *)
+(*            apply convertLetExprSyntax_ActionT_full in H; dest; subst *)
+(*          end. *)
+
+(* Local Ltac destruct_RegT := *)
+(*   repeat match goal with *)
+(*          | H: RegT |- _ => *)
+(*            destruct H as [? [? ?]]; simpl in *; repeat subst; simpl in * *)
+(*          end. *)
+
+(* Local Ltac discharge_init := *)
+(*   repeat econstructor; eauto; simpl; *)
+(*   instantiate (1 := eq_refl); simpl; auto. *)
+
+(* Local Ltac simplify_Ins := *)
+(*   repeat match goal with *)
+(*          | H: In _ (getRules _) |- _ => simpl in H *)
+(*          | H: In _ (getMethods _) |- _ => simpl in H *)
+(*          | H: _ \/ _ |- _ => destruct H *)
+(*          | H: False |- _ => exfalso; apply H *)
+(*          | H: (_, _) = (_, _) |- _ => inv H *)
+(*          | H: (_, _) = ?a |- _ => try subst a *)
+(*          end. *)
+
+(* Ltac discharge_NoSelfCall := *)
+(*   unfold NoSelfCallBaseModule, NoSelfCallRulesBaseModule, NoSelfCallMethsBaseModule; split; auto; intros; *)
+(*   simplify_Ins; *)
+(*   repeat match goal with *)
+(*          | |- NoCallActionT _ (convertLetExprSyntax_ActionT _) => apply LetExprNoCallActionT *)
+(*          | _ => constructor; auto; cbn - [In]; try rewrite (InFilter string_dec); simpl; unfold getBool, not; intros; *)
+(*                 try (rewrite (DisjKey_filter string_dec)); discharge_append *)
+(*          end. *)
+(*   (* unfold NoSelfCallBaseModule, NoSelfCallRulesBaseModule, NoSelfCallMethsBaseModule; split; auto; intros; *) *)
+(*   (* simplify_Ins; *) *)
+(*   (* repeat match goal with *) *)
+(*   (*        | |- NoCallActionT _ (convertLetExprSyntax_ActionT _) => apply LetExprNoCallActionT *) *)
+(*   (*        | _ => constructor; auto; simpl; try intro; try (rewrite (DisjKey_filter string_dec); discharge_append) *) *)
+(*   (*        end. *) *)
+
+
+
+(* Ltac discharge_simulation myRel := *)
+(*   apply simulationGeneral with (simRel := myRel); intros; auto; *)
+(*   repeat match goal with *)
+(*          | H: Forall2 _ _ _ |- _ => inv H; dest *)
+(*          | H: RegT |- _ => destruct H as [? [? ?]]; *)
+(*                            repeat (unfold fst, snd, projT1, projT2 in *; subst) *)
+(*          | _ => discharge_init *)
+(*          | H: myRel _ _ |- _ => inv H; auto *)
+(*          end; [discharge_NoSelfCall | simplify_Ins; discharge_SemAction | simplify_Ins; discharge_SemAction | simplify_Ins | simplify_Ins]. *)
+
+
+(* Notation sz := 5. *)
+
+(* Section Named. *)
+(*   Variable name: string. *)
+(*   Local Notation "^ x" := (name ++ "." ++ x)%string (at level 0). *)
+
+(*     Definition IncrementerImpl := *)
+(*       MODULE_WF { *)
+(*           Register ^"counter" : Bit sz <- Default *)
+(*             with Register ^"counter1" : Bit sz <- Default *)
+(*             with Register ^"isSending" : Bool <- true *)
+                                             
+(*             with Rule ^"send" := *)
+(*             ( Read isSending: Bool <- ^"isSending" ; *)
+(*                 Assert #isSending ; *)
+(*                 Read counter: Bit sz <- ^"counter" ; *)
+(*                 Call "counterVal"(#counter: _); *)
+(*                 Write ^"isSending" <- !#isSending ; *)
+(*                 Retv ) *)
+
+(*             with Rule ^"inc" := *)
+(*               ( Read isSending: Bool <- ^"isSending" ; *)
+(*                   Assert !#isSending ; *)
+(*                   Read counter: Bit sz <- ^"counter" ; *)
+(*                   Write ^"counter" <- #counter + $1; *)
+(*                   Write ^"isSending" <- !#isSending ; *)
+(*                   Retv ) *)
+(*         }. *)
+
+(*   Definition IncrementerSpec := *)
+(*     MODULE_WF { *)
+(*         Register ^"counter" : Bit sz <- Default *)
+(*           with Register ^"counter1" : Bit sz <- Default *)
+                                         
+(*           with Rule ^"send_and_inc" := *)
+(*           ( Read counter: Bit sz <- ^"counter" ; *)
+(*               Call "counterVal"(#counter: _); *)
+(*               Write ^"counter" <- #counter + $1; *)
+(*               Retv) *)
+(*       }. *)
+
+(*   Record Incrementer_invariant (impl spec: RegsT) : Prop := *)
+(*     { counterImpl: word sz ; *)
+(*       isSending: bool ; *)
+(*       implEq : impl = (^"counter", existT _ (SyntaxKind (Bit sz)) counterImpl) *)
+(*                         :: (^"counter1", existT _ (SyntaxKind (Bit sz)) $0) *)
+(*                         :: (^"isSending", existT _ (SyntaxKind Bool) isSending) :: nil ; *)
+(*       specEq : spec = (^"counter", existT _ (SyntaxKind (Bit sz)) *)
+(*                                          (if isSending then counterImpl else counterImpl ^+ $1)) *)
+(*                         :: (^"counter1", existT  _ (SyntaxKind (Bit sz)) $0) *)
+(*                         :: nil *)
+(*     }. *)
+(* End Named. *)
+
+(* Theorem Incrementer_TraceInclusion (name: string) : *)
+(*   TraceInclusion (Base (IncrementerImpl name)) (Base (IncrementerSpec name)). *)
+(* Proof. *)
+(*   discharge_simulation (Incrementer_invariant name). *)
+(*   - right; do 2 (do 2 eexists; repeat split; eauto; simpl in * ). *)
+(*     * repeat (econstructor; eauto; simpl; subst). *)
+(*       unfold key_not_In; unfold not; intros; simpl in *; auto. *)
+(*     * repeat (econstructor; eauto; simpl; subst). *)
+(*       discharge_append. *)
+(*       rewrite wzero_wplus; auto. *)
+(*   - left; split; auto; simpl in *. *)
+(*     repeat (econstructor; eauto; simpl; subst). *)
+(*     rewrite negb_true_iff in *; subst. *)
+(*     rewrite wzero_wplus; simpl; auto. *)
+(* Qed. *)
